
%%%%%%%%%%%%%%%%%%%%%%%%%%%%%%%%%%%%
\begin{table}[!ht]
    \centering
    \begin{tabular}{|l|l|l|}
    \hline
   $\dfrac {\mathrm{d} C}{\mathrm{d} x}=0$ & $\dfrac {\mathrm{d} x}{\mathrm{d} x}=1$ &   $\dfrac {\mathrm{d} \left ( x^n \right )}{\mathrm{d} x}=nx^{n-1}$  \\ \hline  
   $\dfrac {\mathrm{d} \left ( ln (x) \right )}{\mathrm{d} x}=x^{-1}$ & $\dfrac {\mathrm{d} \left ( a^x \right )}{\mathrm{d} x}=a^x ln (a)$ & $\dfrac {\mathrm{d} \left ( e^x \right )}{\mathrm{d} x}=e^x$\\ \hline  
   $\dfrac {\mathrm{d} \left ( \sin ax \right )}{\mathrm{d} x}=a\cos ax$ & $\dfrac {\mathrm{d} \left ( \cos ax \right )}{\mathrm{d} x}=-a\sin ax$ & $\dfrac {\mathrm{d} \left ( \tan ax \right )}{\mathrm{d} x}=\dfrac a{\cos^2 ax}=a\sec^2ax$ \\ \hline
    $\dfrac {\mathrm{d} \left ( \cot x \right )}{\mathrm{d} x}=-\dfrac 1{\sin^2 x}=-\csc^2x$ & $\dfrac {\mathrm{d} \left ( \sec x \right )}
{\mathrm{d} x}=\sec x \tan x$ & $\dfrac {\mathrm{d} \left ( \csc x \right )}
{\mathrm{d} x}=-\csc x \cot x$  \\ \hline
$\dfrac {\mathrm{d} \left ( \arcsin x \right )}{\mathrm{d} x}=\dfrac 1{\sqrt{1-x^2}}$ & $\dfrac {\mathrm{d} \left ( \arccos x \right )}{\mathrm{d} x}=\dfrac {-1}{\sqrt{1-x^2}}$ & $\dfrac {\mathrm{d} \left ( \arctan x \right )}{\mathrm{d} x}=\dfrac 1{1+x^2}$ \\ \hline
$ \dfrac {\mathrm{d} \left ( \arctan x \right )}{\mathrm{d} x}=\dfrac 1{1+x^2}$ & $ \dfrac {\mathrm{d} \left ( arccot\:x \right )}{\mathrm{d} x}=\dfrac {-1}{1+x^2}$ & $ \dfrac {\mathrm{d} \left ( arcsec\:x \right )}{\mathrm{d} x}=\dfrac 1{x\sqrt{x^2-1}}$ \\ \hline
$ \dfrac {\mathrm{d} \left ( arccsc\:x \right )}{\mathrm{d} x}=\dfrac {-1}{x\sqrt{x^2-1}}$ & $ \dfrac {\mathrm{d} \left ( \sinh x \right )}{\mathrm{d} x}=\cosh x$ & $ \dfrac {\mathrm{d} \left ( \cosh x \right )}{\mathrm{d} x}=\sinh x$ \\ \hline
$ \dfrac {\mathrm{d} \left ( \tanh x \right )}{\mathrm{d} x}=\dfrac 1{\cosh^2 x}=sech^2x$ & $ \dfrac {\mathrm{d} \left ( \coth x \right )}{\mathrm{d} x}=-\dfrac 1{\sinh^2 x}=csch^2x$ & $ \dfrac {\mathrm{d} \left ( sech x \right )}{\mathrm{d} x}=-sech\:x \tanh x$ \\ \hline
$ \dfrac {\mathrm{d} \left ( csch x \right )}{\mathrm{d} x}=-csch\:x \coth x$ & $ \dfrac {\mathrm{d} \left ( arcsinh\:x \right )}{\mathrm{d} x}=\dfrac 1{\sqrt{1+x^2}}$ & $ \dfrac {\mathrm{d} \left ( arccosh\:x \right )}{\mathrm{d} x}=\dfrac {-1}{\pm \sqrt{x^2-1}}$ \\ \hline
$ \dfrac {\mathrm{d} \left ( arctanh\:x \right )}{\mathrm{d} x}=\dfrac 1{1-x^2}$ & 
 - & - \\
 \hline
  \end{tabular}
    \caption{Tabla de derivadas}
    \label{tab:Derivadas}
\end{table}








