\begin{table}[h]
\centering
\resizebox{16.5cm}{!}{
\begin{tabular}{|c|c|}
\hline
\multicolumn{1}{|c|}{Propiedad}     & Fórmula \\ \hline
Definición	& $	\dst F(s)=\mathcal {L} \{ f(t) \}= \int_0^{\infty} e^{-st}f(t) \dd t $  \\ \hline
Linealidad	& $	\mathcal {L} \{ a \cdot f(t) +b \cdot g(t)\}= a \cdot \mathcal {L} \{f(t) \}+b \cdot \mathcal {L} \{ g(t)\}$ \\ \hline
Derivación 
& \ensuremath{   
\begin{array}{c}
  \mathcal {L} \{ f'(t) \}=s \mathcal {L} \{ f(t) \}-f(0)\\ 
  \mathcal {L} \{ f''(t) \}=s^2 \\ 
  \mathcal {L} \{ f(t) \}-s f(0)-f'(0) \\ 
  \mathcal {L} \{ f^{(n)}(t) \}= s^n \mathcal {L} \{ f(t) \}-s^{n-1} f(0)-\ldots-f^{(n-1)}(0) 
  \\ \mathcal {L} \{ f^{(n)}(t) \}= s^n \mathcal {L} \{ f(t) \}-\dst \sum_{i=1}^n s^{n-i}f^{(i-1)}(0)
\end{array}  
} \\ \hline
Integración	& $	\mathcal {L} \{ \int_{0-}^t f(\tau) \dd \tau \}=\dfrac 1s \mathcal {L} \{ f(t) \}$ \\ \hline
Dualidad& $		\mathcal {L} \{ t \cdot f(t) \}=-F'(s)$ \\ \hline
Desplazamiento de frecuencia	& $	\mathcal {L} \{ e^{at}f(t) \}=F(s-a)$ \\ \hline
Desplazamiento temporal	
& \ensuremath{   
\begin{array}{c}
  \mathcal {L} \{ f(t-a) \cdot u(t-a) \}=e^{-as} F(s) \\ \mathcal {L}^{-1} \{ e^{-as} F(s) \}=f(t-a) \cdot u(t-a) \\ u(t-a)=\left\{ \begin{array}{cl}0 & \text{si}\ t < a \\1 & \text{si}\ t \ge a \end{array}\right.
\end{array}  
} \\ \hline

Convolución	& $	\mathcal {L} \{ f(t) \cdot g(t) \}=F(s) \cdot G(s)   $ \\ \hline

\end{tabular}}
\caption{Propiedades de Transformadas de Laplace}
\label{tab:prop-transf-laplace}
\end{table}